---
title: "hw4"
author: "Hanbei Xiong"
format: html
editor: visual
---

# Problem 1

![](images/WeChatc3063296176c7f79bfe5d0c2824824cb.png)

**Answer:**

Assume A and B should both have uniform distribution

$A\sim U(1,2)$ and $B\sim U(1,2)$

$f_{A,B}(a,b)=1$ for $1\leq a \leq 2$ and $1\leq b \leq 2$

Let X = B-A

Then:

$$
X=
\left\{
    \begin{array}{ll}
        0 & \text{if } B-A\leq 0 \\
        B-A & \text{if } B-A>0
    \end{array}
\right.
$$

$$
F_X(x)=
\left\{
    \begin{array}{ll}
        0 & \text{if } x\leq 0 \\
        P(B-A>0)+P(B-A\leq 0) & \text{if } 0<x<1 \\
        1 & \text{if } x\geq 1
    \end{array}
\right.
$$

If we draw the graph where x-axis represented A and y-axis represented B, the support of X is a square form by $1\leq a \leq 2$ and $1\leq b \leq 2$. We can use the 1 minus the probability of landing on area of upper left triangle to represent the distribution of length of time that A waits for B. Here is the distribution:

$$
F_X(x)=
\left\{
    \begin{array}{ll}
        0 & \text{if } x\leq 0 \\
        1-\int_{1}^{2-x}\int_{a+x}^{2}1dbda = 1-\int_{1}^{2-x} (2-a-x)da = 1-[(2-x)a-\frac{a^2}{2}]\Big|_{1}^{2-x}=1-(2-x)^2+\frac{(2-x)^2}{2}+(2-x)-\frac{1}{2}=-(2-x)^2/2-x+\frac{5}{2}& \text{if } 0<x<1 \\
        1 & \text{if } x\geq 1
    \end{array}
\right.
$$

# Problem 2

![](images/WeChatd73b5ee85433479248462a20ffbb64fc.png)

**(a) Answer:**

X and Y are not independent since their supports are not rectangular support.

**(b) Answer:**

$f_{Y}(y)=\int_{-\sqrt{y}}^{\sqrt{y}}\frac{21}{4}x^2y dx=\frac{7}{4}x^3y\Big|_{-\sqrt{y}}^{\sqrt{y}}=\frac{7}{2}y^\frac{5}{2}$ for $0\leq y \leq 1$

**(c) Answer:**

$E(Y)=\int_{-\infty}^{\infty} yf_{Y}(y)dy=\int_{0}^{1} \frac{7}{2}y^{\frac{7}{2}}dy=\frac{7}{9}y^{\frac{9}{2}}\Big|_{0}^{1}=\frac{7}{9}$

$E(Y^2)=\int_{-\infty}^{\infty} y^2f_{Y}(y)dy=\int_{0}^{1} \frac{7}{2}y^{\frac{9}{2}}dy=\frac{7}{11}y^{\frac{11}{2}}\Big|_{0}^{1}=\frac{7}{11}$

$Var(Y)=E(Y^2)-E(Y)^2=\frac{7}{11}-\frac{49}{81}\approx 0.0314$

**(d) Answer:**

$F_{Y}(y)=\int_{0}^{y}\frac{7}{2}z^\frac{5}{2}dz=y^\frac{7}{2}$, $0\leq y \leq 1$

**(e) Answer:**

We let y=x and graph it out. By selecting a random point like (1,0), we can tell the point is below the line. We can also let $x^2=y$ and graph it on the same graph. We can tell the support of the joint pdf is the area between this parabola. Hence, we are looking for the area between these two functions.

The graph looks like this:

![](images/WeChat5722c684a3f12fb955bf625e8c9eb68f.png){width="304"}

$P(X\geq Y)=\int_{0}^{1}\int_{x^2}^{x}\frac{21}{4}x^2ydydx=\int_{0}^{1}\frac{21}{8}x^2y^2\Big|_{x^2}^{x}dx=\int_{0}^{1}\frac{21}{8}x^2(x^2-x^4)dx=\frac{21}{8}\int_{0}^{1}x^4-x^6dx=\frac{21}{8}[\frac{1}{5}x^5-\frac{1}{7}x^7]\Big|_{0}^{1}=\frac{21}{8}[\frac{1}{5}-\frac{1}{7}]=\frac{21}{8}[\frac{2}{35}]=\frac{3}{20}$

# Problem 3

![](images/WeChat9c62630d53a1417209b0164d7ac7ce96.png)

**(a) Answer:**

We can find $x_1=u(y_1,y_2)$ and $x_2=v(y_1,y_2)$

Since

$Y_1=X_1+X_2$ and $Y_2=X_1-X_2$

$\Rightarrow X_1=\frac{Y_1+Y_2}{2}$ and $X_2=\frac{Y_1-Y_2}{2}$

We can also transform the support of $X_1$ and $X_2$ to the support of $Y_1$ and $Y_2$.

We have $0<X_1<1$ and $0<X_2<1$

It becomes:

$0<\frac{Y_1+Y_2}{2}<1$ and $0<\frac{Y_1-Y_2}{2}<1$

The inequality can be saperated into four parts:

$y_2>-y_1$ and $y_2<y_1$ and $y_2<2-y_1$ and $y_2>y_1-2$

By setting inequality to equality, we can find the support of $Y_1$ and $Y_2$:

![](images/WeChatde6c5b9784b3d21ccab0de0ca18586c5.png){width="423"}

The horizontal axis is $y_1$ and the vertical axis is $y_2$. By pluging in point as (1,0), we know the support of joint distribution of $Y_1$ and $Y_2$ is the area between these lines.

$$
|J|=|det\begin{bmatrix}
            \frac{\partial x_1}{\partial y_1} & \frac{\partial x_1}{\partial y_2} \\
            \frac{\partial x_2}{\partial y_1} & \frac{\partial x_2}{\partial y_2} \\
        \end{bmatrix}|=|det\begin{bmatrix}
            \frac{1}{2} & \frac{1}{2} \\
            \frac{1}{2} & -\frac{1}{2} \\
        \end{bmatrix}|=\frac{1}{2}
$$

$f_{Y_1,Y_2}(y_1,y_2)=f_{X_1,X_2}(x_1,x_2)|J|=\frac{1}{2}$

**(b) Answer:**

$$ 
f_Y(y_1)=
\begin{cases}
\int_{-y_1}^{y_1}\frac{1}{2}dy_2=y_1 & \text{if } 0<y_1<1 \\
\int_{y_1-2}^{-y_1+2}\frac{1}{2}dy_2=-y_1+2 & \text{if } 1<y_1<2
\end{cases} 
$$

# Problem 4

![](images/WeChat66bc7f0f3dd1727b02712db4aa3e767a.png)

**(a) Answer:**

$P(X=x)=f_{X}(x)=\sum_{y\in S_y} g(x)h(y)=g(x)\sum_{y\in S_y}h(y)$

$P(Y=y)=f_{Y}(y)=\sum_{x\in S_x} g(x)h(y)=h(y)\sum_{x\in S_x}g(x)$

**(b) Answer:**

$(\sum_{x\in S_x}g(x))(\sum_{y\in S_y}h(x))=\sum_{x\in S_x,y\in S_y}g(x)h(x)=\sum_{x\in S_x,y\in S_y}P(X=x,Y=y)=1$

$P(X=x)P(Y=y)=(g(x)\sum_{y\in S_y}h(y))(h(y)\sum_{x\in S_x}g(x))=g(x)h(y)(\sum_{y\in S_y}h(y))(\sum_{x\in S_x}g(x))=g(x)h(y)=P(X=x,Y=y)$

Hence, X and Y are independent.

# Problem 5

![](images/WeChatefc5d74c8906d2758af4fbbf6bf28a06.png)

**Answer:**

Given:

$Pr(X=1)=p$

$Pr(X=0)=1-p$

$Pr(Y = 1|X=1)=r$

$Pr(Y = 0|X=0)=s$

We know:

$Var(Y)=E(Y^2)-E(Y)^2$

$E(Y)=1*Pr(Y=1)+0*Pr(Y=0)=1*(Pr(Y=1|X=1)Pr(X=1)+Pr(Y=1|X=0)Pr(X=0))=rp+(1-s)(1-p)$

$E(Y^2)=1^2*Pr(Y=1)+0^2*Pr(Y=0)=1^2*(Pr(Y=1|X=1)Pr(X=1)+Pr(Y=1|X=0)Pr(X=0))=rp+(1-s)(1-p)$

$Var(Y)=rp+(1-s)(1-p)-[rp+(1-s)(1-p)]^2$
