---
title: "hw6"
author: "Hanbei Xiong"
format: html
editor: visual
---

## Question 1

![](images/WeChata5d412f1df4966bb1b5a21d980a0f94d.png)

**(a) Answer:**

$Z_i=\frac{X_i-i}{\sqrt{i^2}}=\frac{X_i-i}{i}$ for i = 1, 2, 3

$Z_i\sim N(0,1)$

$\sum_{i=1}^{3}(\frac{X_i-i}{i})^2 \sim \chi^2(3)$

**(b) Answer:**

$\sum_{i=1}^{2}(\frac{X_i-i}{i})^2\sim \chi^2(2)$

By independence of $X_1$, $X_2$, and $X_3$,

$\frac{X_1-1}{\sqrt{\sum_{i=2}^{3}(\frac{X_i-i}{i})^2/2}}\sim t_2$

**(c) Answer:**

$(X_1-1)^2\sim \chi^2(1)$

$\frac{\chi^2(1)/1}{\chi^2(2)/2}\sim F_{1,2}$

By independence of $X_1$, $X_2$, and $X_3$,

$\frac{(X_1-1)^2}{\sum_{i=2}^{3}(\frac{X_i-i}{i})^2/2}\sim F_{1,2}$

## Question 2

![](images/WeChat388cc619e502d80a098fc53dc1841865.png) **Answer:**

By independence of X and Y,

$M_W(t)=M_{X^2+2Y^2}(t)=E[e^{X^2t+2Y^2t}]=E[e^{X^2t}]E[e^{2Y^2t}]=M_{X^2}(t)M_{Y^2}(2t)$

Since X and Y are iid normal(0,1)

$X^2 \sim \chi^2(1)$

$Y^2 \sim \chi^2(1)$

$M_{X^2}(t)=\frac{1}{(1-2t)^{1/2}}$, t\<1/2

$M_{Y^2}(2t)=\frac{1}{(1-4t)^{1/2}}$, t\<1/4

$M_W(t)=M_{X^2}(t)M_{Y^2}(2t)=\frac{1}{(1-2t)^{1/2}}\frac{1}{(1-4t)^{1/2}}$, t\<1/4

Since it is not in the shape of the MGF of chisquare distribution, we can conclude that W does not follow a chisquare distribution.

## Question 3

![](images/WeChat1f83d7be1de99c5ef79d1d59ab798d2f.png)

**Answer:**

$M_Y(t)=E[e^{X_1t+X^2t}]=M_{X_1}(t)M_{X^2}(t)$

$M_{X_2}(t)=\frac{M_Y(t)}{M_{X_1}(t)}$

Since $Y \sim Poisson(\mu)$ and $X_1 \sim Poisson(\mu_1)$,

$M_Y(t)=e^{\mu(e^t-1)}$ $\forall t$

$M_{X_1}(t)=e^{\mu_1(e^t-1)}$ $\forall t$

$M_{X_2}(t)=\frac{M_Y(t)}{M_{X_1}(t)}=e^{\mu(e^t-1)-\mu_1(e^t-1)}=e^{(\mu-\mu_1)(e^t-1)}$ $\forall t$

Therefore, $X_2 \sim Poisson(\mu-\mu_1)$

## Question 4

![](images/WeChatb345dc551605e1a80824ee34feabb8d1.png)

**(a) Answer:**

Since $\sum r^x=\frac{1}{1-r}$ for \|r\| \< 1,

$M_X(t)=E[e^{tX}]=\sum_{x=0}^{\infty}e^{tx}p(1-p)^x = p\sum_{x=0}^{\infty}e^{tx}(1-p)^x=p\sum_{x=0}^{\infty}(e^{t}(1-p))^x=\frac{p}{1-e^{t}(1-p)}$

To find the bound of t,

$|e^{t}(1-p)|<1 \Rightarrow e^{t}(1-p)<1\Rightarrow t+log(1-p)<0\Rightarrow t<-log(1-p)$

**(b) Answer:**

Let $\psi_X(t)=logM_X(t)=log(p)-log(1-e^t(1-p))$

$\mu_X=\psi_X'(t)\Big|_{t=0}=\frac{e^t(1-p)}{1-e^t(1-p)}\Big|_{t=0}=\frac{1-p}{p}$

$\sigma^2_X=\psi_X''(t)\Big|_{t=0}=\frac{(1-p)e^t\{1-(1-p)e^t\}+(1-p)^2e^{2t}}{\{1-e^t(1-p\}^2}\Big|_{t=0}=\frac{(1-p)p+(1-p)^2}{p^2}=\frac{1-p}{p^2}$

**(c) Answer:**

By central limit theorem:

$\frac{\sqrt{n}(\bar{X}-\mu_x)}{\sigma_x}\sim N(0,1)$

$E[\sqrt{n}(\bar{X}-\mu_x)]=0$

$Var[\sqrt{n}(\bar{X}-\mu_x)]=\sigma^2_x$

$\sqrt{n}(\bar{X}-\mu_x)\sim N(0,\sigma^2_x)$

## Question 5

![](images/WeChatdf0bf31c249a181e2de59fee7310b334.png)

**Answer:**

$E[e^{Y_1Y_2t}]=E_{Y_2}\{E[e^{Y_1Y_2t}|Y_2]\}$

Let $Y_2=y_2$

$E[e^{Y_1Y_2t}|Y_2=y_2]=E[e^{Y_1y_2t}|Y_2=y_2]=E[e^{Y_1y_2t}]=M_{Y_1}(y_2t)$

Since $Y_1\sim N(0,1)$

$M_{Y_1}(y_2t)=e^{\frac{1}{2}y_2^2t^2}$ where $-\infty<t<\infty$

Replace $y_2$ with $Y_2$

$E_{Y_2}[e^{\frac{1}{2}Y_2^2t^2}]=M_{Y_2^2}(\frac{1}{2}t^2)$

Since $Y_2\sim N(0,1)$, we have $Y_2^2\sim \chi^2(1)$

$M_{Y_2^2}(\frac{1}{2}t^2)=\frac{1}{(1-2\frac{1}{2}t^2)^{1/2}}=\frac{1}{(1-t^2)^{1/2}}$

The support of t can be found below:

$\frac{t^2}{2} <\frac{1}{2}\Rightarrow -1<t<1$

$M_Y(t)=\frac{1}{(1-t^2)^{1/2}}$

## Question 6

![](images/WeChat03dcf00811e5b60105f1c407d7c3daa2.png)

**(a) Answer:**

$Y=e^X\Rightarrow logY=X$

$\infty < X < \infty \Rightarrow 0 < Y < \infty$

$f_{X}(x)=\frac{1}{\sqrt{2\pi}\sigma}e^{-\frac{(x-\mu)^2}{2\sigma^2}}$ with support: $-\infty<x<\infty$

$|\frac{dx}{dy}|=|\frac{dlogy}{dy}|=|\frac{1}{y}|=\frac{1}{y}$

$f_Y(y)=f_X(logy)|\frac{dx}{dy}|=\frac{1}{\sqrt{2\pi}\sigma}e^{-\frac{(log(y)-\mu)^2}{2\sigma^2}}\frac{1}{y}$ with support: $0<y<\infty$

**(b) Answer:**

$E[Y^k]=E[e^{Xk}]=M_X{(k)}=e^{k\mu+\frac{k^2\sigma^2}{2}}$ for all k
