---
title: "hw5"
author: "Hanbei Xiong"
format: html
editor: visual
---

# Problem 1

![](images/WeChate321ba9f5158dfa487a5e9b9eacdbe03.png)

**Answer:**

Chebychev Inequality:

Set up the equation as $P(|\bar{X}-\mu|< a) \geq 0.9$, we are trying to find a

$P(|\bar{X}-\mu|< a)=1-P(|\bar{X}-\mu|\geq a)\geq 0.9$

$P(|\bar{X}-\mu|\geq a)\leq 0.1$

By Chebychev's inequality, $P(|\bar{X}-\mu|\geq a)\leq \frac{\sigma^2}{na^2}=0.1$

$a^2= \frac{\sigma^2}{0.1n}=\frac{9}{0.1\times 100}=0.9$

Since a is nonnegative, $a=\sqrt{0.9}\approx 0.9487$

Here is the limit:

$-0.9487<\bar{X}-\mu <0.9487$

Central Limit Theorem:

Set up the equation as $P(\frac{|\bar{X}-\mu|}{\sigma/\sqrt{n}}\leq a) \geq 0.9$, 

By z-score table,

$P(\frac{|\bar{X}-\mu|}{\sigma/\sqrt{n}}\leq 1.645) \geq 0.9$

$P(|\bar{X}-\mu|\leq 1.645\times \sqrt{\frac{\sigma^2}{n}}) = 0.9$

$P(|\bar{X}-\mu|\leq 1.645\times \sqrt{\frac{9}{100}}) = 0.9$

$P(|\bar{X}-\mu|\leq 0.494) = 0.9$

Here is the limit:

$-0.494\leq \bar{X}-\mu \leq 0.494$

# Problem 2

![](images/WeChat2786dfac7d92e153fd756387dc5c2e6b.png)

**Answer: **

$E(X)=\int_{0}^{1}x(2(1-x))dx=\int_{0}^{1}(2x-2x^2)dx=(x^2-\frac{2}{3}x^3)\Big|_{0}^{1}=\frac{1}{3}$

$E(X^2)=\int_{0}^{1}x^2(2(1-x))dx=\int_{0}^{1}(2x^2-2x^3)dx=(\frac{2}{3}x^3-\frac{1}{2}x^4)\Big|_{0}^{1}=\frac{1}{6}$

$Var(X)=E(X^2)-E(X)^2=\frac{1}{6}-(\frac{1}{3})^2=\frac{1}{18}$

$P(\sum_{i=1}^{72}X_i<28)=P(\frac{\sum_{i=1}^{72}X_i}{72}<\frac{28}{72})=P(\bar{X}<\frac{7}{18})=P(\frac{\bar{X}-\mu}{\sigma/\sqrt{n}}<\frac{\frac{7}{18}-\frac{1}{3}}{\sqrt{\frac{1}{18}/72}})=P(Z<\frac{\frac{7}{18}-\frac{1}{3}}{\sqrt{\frac{1}{18}/72}})=P(Z<2)=0.9772$


# Problem 3

![](images/WeChat12c0895b79f5a4373f5a03dca6c2e1b7.png)

**(a) Answer:**

```{=tex}
\begin{align*}
E(e^{X_1t_1+X_2t_2})&=\int_{0}^{\infty}\int_{0}^{x_2}e^{X_1t_1+X_2t_2}\times 2e^{-x_2}e^{-x_1}dx_1dx_2\\
&=2\int_{0}^{\infty}\int_{0}^{x_2}e^{x_1(t_1-1)}e^{x_2(t_2-1)}dx_1dx_2\\
&=2\int_{0}^{\infty}\frac{1}{t_1-1}e^{x_2(t_1+t_2-2)}-\frac{1}{t_1-1}e^{x_2(t_2-1)}dx_2\\
&=2(\frac{1}{t_1-1}\frac{1}{t_1+t_2-2}e^{x_2(t_1+t_2-2)}-\frac{1}{(t_1-1)(t_2-1)}e^{x_2(t_2-1)})\Big|_{0}^{\infty}\\
&=-\frac{2}{(t_1-1)(t_1+t_2-2)}+\frac{1}{(t_1-1)(t_2-1)} \text{ with support: } t_1<1 \text{ and } t_2<1
\end{align*}
```

**(b) Answer:**

We will solve this problem by first finding the cdf of Y

For simplicity of notation, I will use $Y_1=Y$ 

Let $Y_1=X_2-X_1$, $Y_2=X_1$

The inverse functions are $X_1=Y_2$, $X_2=Y_1+Y_2$

The Jacobian is $\frac{\partial(X_1,X_2)}{\partial(Y_1,Y_2)}=\begin{vmatrix} \frac{\partial X_1}{\partial Y_1} & \frac{\partial X_1}{\partial Y_2} \\ \frac{\partial X_2}{\partial Y_1} & \frac{\partial X_2}{\partial Y_2} \end{vmatrix}=\begin{vmatrix} 0 & 1 \\ 1 & 1 \end{vmatrix}=1$

$f_{Y_1,Y_2}(y_1,y_2)=f_{X_1,X_2}(y_2,y_1+y_2)|\frac{\partial(X_1,X_2)}{\partial(Y_1,Y_2)}|=2e^{-y_2}e^{-(y_1+y_2)}$

The support of $Y_1$ is $0<y_1<\infty$, and the support of $Y_2$ is $0<y_2<\infty$

The cdf of $Y_1$ is $F_{Y_1}(y_1)=P(Y_1\leq y_1)=\int_{0}^{y_1}\int_{0}^{\infty}2e^{-y_2}e^{-(y_1+y_2)}dy_2dy_1=-2e^{-y_1}+2$ with support $0<y_1<\infty$

$M_{Y_1}(t)=E(e^{Y_1t})=\int_{0}^{\infty}e^{y_1t}(-2e^{-y_1}+2)dy_1=-(\frac{2}{t-1}+\frac{2}{t})$ for $t<0$

# Problem 4

![](images/WeChat5f1c95ea99065e3c0db125829c2365b6.png)

**(a) Answer:**

$E(S)=E_{N}\{E(S|N)\}=E_{N}\{E(\sum_{i=1}^{N}X_i|N)\}$

Let N=n, 

$E(S|N=n)=E(\sum_{i=1}^{N}X_i|N=n)=E(\sum_{i=1}^{n}X_i|N=n)=E(\sum_{i=1}^{n}X_i)=\sum_{i=1}^{n}E(X_i)=n\mu_x$

Then, $E(S|N)=N\mu_x$

$E(S)=E_{N}\{E(S|N)\}=E_{N}\{N\mu_x\}=E_N(N)\mu_x=\mu_N\mu_x$

$Var(S)=E_{N}\{Var(S|N)\}+Var_{N}\{E(S|N)\}$

let N=n,

$Var(S|N=n) = Var(\sum_{i=1}^{N}X_i|N=n)=Var(\sum_{i=1}^{n}X_i|N=n)=Var(\sum_{i=1}^{n}X_i)=\sum_{i=1}^{n}Var(X_i)=n\sigma_x^2$

Then, $Var(S|N)=N\sigma_x^2$

$Var(S)=E_{N}\{Var(S|N)\}+Var_{N}\{E(S|N)\}=E_{N}\{N\sigma_x^2\}+Var_{N}\{N\mu_x\}=E_N(N)\sigma_x^2+Var_N(N)\mu_x^2=\mu_N\sigma_x^2+\sigma_N^2\mu_x^2$

**(b) Answer:**

$M_S(t)=E(e^{St})=E_{N}\{E(e^{St}|N)\}=E_{N}\{E(e^{\sum_{i=1}^{N}X_i}|N)\}$

let N=n,

$E(e^{\sum_{i=1}^{N}X_i}|N=n)=E(e^{\sum_{i=1}^{n}X_i}|N=n)=E(e^{\sum_{i=1}^{n}X_i})=M_X^n(t)$

Then, $E(e^{St}|N)=M_X^N(t)$

$E(e^{St})=E_{N}\{E(e^{St}|N)\}=E_{N}\{M_X^N(t)\}=E_{N}\{e^{NlogM_X(t)}\}=M_N(logM_X(t))$

# Problem 5

![](images/WeChatba5ab521a6857aeb1bd6841300bce3e8.png)

**Answer:**

```{=tex}
\begin{align*}
f(x) = \frac{d}{dx}F(x) = \frac{d}{dx}P(1-e^{-2}) = 2e^{-2x} \text{ for } x>0
\end{align*}
```
```{=tex}
\begin{align*}
M_X(t) &= E(e^{Xt})\\
&= \int_{0}^{\infty}e^{xt}f(x)dx\\
&= \int_{0}^{\infty}e^{xt}2e^{-2x}dx\\
&= 2\int_{0}^{\infty}e^{x(t-2)}dx\\
&= \frac{2}{t-2}e^{x(t-2)}\Big|_{0}^{\infty}\\
&= -\frac{2}{t-2} \text{ for } t<2
\end{align*}
```
```{=tex}
\begin{align*}
Cov(X_1+2X_2, X_1-X_2) &= E((X_1+2X_2)(X_1-X_2)) - E(X_1+2X_2)E(X_1-X_2)\\
&= E(X_1^2+2X_1X_2-X_1X_2-2X_2^2) - (E(X_1)+2E(X_2))(E(X_1)-E(X_2))\\
&= E(X_1^2) + E(X_1)E(X_2) - 2E(X_2^2) - E(X_1)^2 - 2E(X_1)E(X_2) + E(X_1)E(X_2)+2E(X_2)^2\\
&= (E(X_1^2) - E(X_1)^2) - 2(E(X_2^2) - E(X_2)^2)
\end{align*}
```
```{=tex}
\begin{align*}
E(X_1^2) &= \frac{d^2}{dt^2}M_{X_1}(t)\Big|_{t=0}\\
&= \frac{d^2}{dt^2}(-\frac{2}{t-2})\Big|_{t=0}\\
&= \frac{2}{(t-2)^2}\Big|_{t=0}\\ 
&= \frac{1}{2}
\end{align*}
```
$E(X_1)^2 = (\frac{d}{dt}M_{X_1}(t)\Big|_{t=0})^2=(\frac{2}{(t-2)^2}\Big|_{t=0})^2=\frac{1}{4}$

Since $X_1$ and $X_2$ have the same cdf, $E(X_1)^2=E(X_2)^2=\frac{1}{4}$ and $E(X_2^2)=E(X_1^2)=\frac{1}{2}$

$Cov(X_1+2X_2, X_1-X_2) = \frac{1}{2} - \frac{1}{4} = \frac{1}{4}$

# Problem 6

![](images/WeChat9502520712662030aaee140764baa362.png)

**Answer:**

```{=tex}
\begin{align*}
P(X\geq a)&=P(Xt\geq at)\\
&= P(e^{Xt}\geq e^{at})\\
&\leq \frac{E(e^{Xt})}{e^{at}}\\
&= e^{-at}M_X(t) \text{ , } \forall 0<t<h
\end{align*}
```
